src/Raft.thy
@@ -61,14 +61,120 @@ qed
 definition (in raft) valid_params where
   "valid_params n i \<equiv> (n < length all_states \<and> i < number_of_nodes)"
 
-lemma (in raft) valid_params_length_previous: "valid_params (n + 1) i \<Longrightarrow> valid_params n i"
-  by (meson add_lessD1 valid_params_def)
+lemma (in raft) valid_params_length_smaller: "\<lbrakk> n > m; valid_params n i \<rbrakk> \<Longrightarrow> valid_params m i"
+  by (metis add_lessD1 less_imp_add_positive valid_params_def)
 
-lemma (in raft) state_length_invariant: "valid_params n 0 \<Longrightarrow> length (all_states ! n) = number_of_nodes"
+lemma (in raft) state_length_invariant: "valid_params n i \<Longrightarrow> length (all_states ! n) = number_of_nodes"
   apply (induct n)
   apply (metis hd_0th initial_state raft.valid_params_def raft_axioms repeat_length)
-  apply (metis Suc_eq_plus1 state_length_invariant_for_transition transition valid_params_length_previous)
-  done
+  by (metis Suc_eq_plus1 lessI raft.valid_params_length_smaller raft_axioms state_length_invariant_for_transition transition)
+
+lemma (in raft) message_is_finite: "valid_params n i \<Longrightarrow> finite (all_messages ! n)"
+  apply (induct n)
+  apply (simp add: valid_params_def)
+  apply (metis finite.intros(1) hd_0th initial_message length_greater_0_conv state_message_sync)
+  by (metis Suc_eq_plus1 lessI raft.valid_params_length_smaller raft_axioms transition transition_message_preserves_finite)
+
+lemma (in raft) transision_preserves_valid_sender_and_receiver:
+  "\<lbrakk> (\<sigma>,m) \<rightarrow> (\<sigma>',m'); x \<in> m'; length \<sigma> > 0 \<rbrakk>
+  \<Longrightarrow> x \<in> m \<or> ((node_of (sender x)) < length \<sigma> \<and> (node_of (receiver x)) < length \<sigma>)"
+  apply (cases rule: transition.cases)
+  apply simp
+proof-
+  fix \<sigma>'' \<sigma>''' ms ms' target
+  assume "(\<sigma>, m) \<rightarrow> (\<sigma>', m')" "x \<in> m'" "length \<sigma> > 0" "(\<sigma>, m) = (\<sigma>'', ms)" "(\<sigma>', m') = (\<sigma>''', ms')" "TR_condition_start_election \<sigma>'' \<sigma>''' ms ms' target"
+
+  have "\<exists>index term. ms' = ms \<union> {message (node target) (node i) (request_vote (node target) index term) (currentTerm (\<sigma>''' ! target)) |i. i \<le> length \<sigma>'' - Suc 0 \<and> i \<noteq> target}"
+    using \<open>TR_condition_start_election \<sigma>'' \<sigma>''' ms ms' target\<close>
+    by (auto simp add: TR_condition_start_election_def)
+  hence "\<exists>index term. x \<in> ms \<union> {message (node target) (node i) (request_vote (node target) index term) (currentTerm (\<sigma>''' ! target)) |i. i \<le> length \<sigma>'' - Suc 0 \<and> i \<noteq> target}"
+    using \<open>(\<sigma>', m') = (\<sigma>''', ms')\<close> \<open>x \<in> m'\<close> by blast
+  hence "x \<in> ms \<or> node_of (sender x) = target \<and> node_of (receiver x) \<le> length \<sigma>'' - 1"
+    by auto
+  hence "x \<in> ms \<or> node_of (sender x) = target \<and> node_of (receiver x) < length \<sigma>''"
+    by (metis Suc_diff_1 \<open>(\<sigma>, m) = (\<sigma>'', ms)\<close> \<open>0 < length \<sigma>\<close> less_Suc_eq_le old.prod.inject)
+
+  have "target < length \<sigma>''"
+    using \<open>TR_condition_start_election \<sigma>'' \<sigma>''' ms ms' target\<close>
+    by (simp add: TR_condition_start_election_def)
+
+  show "x \<in> m \<or> node_of (sender x) < length \<sigma> \<and> node_of (receiver x) < length \<sigma>"
+    using \<open>(\<sigma>, m) = (\<sigma>'', ms)\<close> \<open>target < length \<sigma>''\<close> \<open>x \<in> ms \<or> node_of (sender x) = target \<and> node_of (receiver x) < length \<sigma>''\<close> le_less by blast
+next
+  fix \<sigma>'' \<sigma>''' ms ms' ma r s t vg
+  show "(\<sigma>, m) \<rightarrow> (\<sigma>', m') \<Longrightarrow>
+       x \<in> m' \<Longrightarrow>
+       0 < length \<sigma> \<Longrightarrow>
+       (\<sigma>, m) = (\<sigma>'', ms) \<Longrightarrow>
+       (\<sigma>', m') = (\<sigma>''', ms') \<Longrightarrow>
+       TR_condition_request_vote_resp \<sigma>'' \<sigma>''' ms ms' ma r s t vg \<Longrightarrow> x \<in> m \<or> node_of (sender x) < length \<sigma> \<and> node_of (receiver x) < length \<sigma>"
+    apply (simp add: TR_condition_request_vote_resp_def)
+    by (metis insertE message.sel(1) message.sel(2) node.sel)
+next
+  show "\<And>\<sigma>'' \<sigma>''' ms ms' target.
+       (\<sigma>, m) \<rightarrow> (\<sigma>', m') \<Longrightarrow>
+       x \<in> m' \<Longrightarrow>
+       0 < length \<sigma> \<Longrightarrow>
+       (\<sigma>, m) = (\<sigma>'', ms) \<Longrightarrow>
+       (\<sigma>', m') = (\<sigma>''', ms') \<Longrightarrow>
+       TR_condition_promote_to_leader \<sigma>'' \<sigma>''' ms ms' target \<Longrightarrow> x \<in> m \<or> node_of (sender x) < length \<sigma> \<and> node_of (receiver x) < length \<sigma>"
+    by (simp add: TR_condition_promote_to_leader_def)
+next
+  show "\<And>\<sigma>'' \<sigma>''' ms ms' s r.
+       (\<sigma>, m) \<rightarrow> (\<sigma>', m') \<Longrightarrow>
+       x \<in> m' \<Longrightarrow>
+       0 < length \<sigma> \<Longrightarrow>
+       (\<sigma>, m) = (\<sigma>'', ms) \<Longrightarrow>
+       (\<sigma>', m') = (\<sigma>''', ms') \<Longrightarrow> TR_condition_append_entry \<sigma>'' \<sigma>''' ms ms' s r \<Longrightarrow> x \<in> m \<or> node_of (sender x) < length \<sigma> \<and> node_of (receiver x) < length \<sigma>"
+    apply (simp add: TR_condition_append_entry_def)
+    apply auto
+    done
+next
+  show "\<And>\<sigma>'' \<sigma>''' ms ms' leadersLog prevLogTerm prevLogIndex t success r s.
+       (\<sigma>, m) \<rightarrow> (\<sigma>', m') \<Longrightarrow>
+       x \<in> m' \<Longrightarrow>
+       0 < length \<sigma> \<Longrightarrow>
+       (\<sigma>, m) = (\<sigma>'', ms) \<Longrightarrow>
+       (\<sigma>', m') = (\<sigma>''', ms') \<Longrightarrow>
+       TR_condition_append_entry_resp \<sigma>'' \<sigma>''' ms ms' leadersLog prevLogTerm prevLogIndex t success r s \<Longrightarrow>
+       x \<in> m \<or> node_of (sender x) < length \<sigma> \<and> node_of (receiver x) < length \<sigma>"
+    apply (simp add: TR_condition_append_entry_resp_def)
+    by (metis insertE message.sel(1) message.sel(2) node.sel)
+qed
+
+lemma (in raft) all_messages_contains_valid_messages: "\<lbrakk> valid_params n i; m \<in> all_messages ! n \<rbrakk> \<Longrightarrow> valid_params n (node_of (sender m)) &&& valid_params n (node_of (receiver m))"
+  apply (induct n arbitrary: m)
+  using hd_conv_nth initial_message state_message_sync valid_params_def apply auto[1]
+  using hd_conv_nth initial_message state_message_sync valid_params_def apply auto[1]
+proof-
+  fix n m
+  assume "(\<And>m. valid_params n i \<Longrightarrow> m \<in> all_messages ! n \<Longrightarrow> valid_params n (node_of (sender m)))"
+    "(\<And>m. valid_params n i \<Longrightarrow> m \<in> all_messages ! n \<Longrightarrow> valid_params n (node_of (receiver m)))"
+    "valid_params (Suc n) i" "m \<in> all_messages ! Suc n"
+  have "(all_states ! n, all_messages ! n) \<rightarrow> (all_states ! (n + 1), all_messages ! (n + 1))"
+    by (simp add: transition)
+
+  hence "m \<in> all_messages ! n \<or> node_of (sender m) < length (all_states ! n) \<and> node_of (receiver m) < length (all_states ! n)"
+    apply (rule transision_preserves_valid_sender_and_receiver)
+    using \<open>m \<in> all_messages ! Suc n\<close> apply auto
+    by (metis Suc_eq_plus1 \<open>(all_states ! n, all_messages ! n) \<rightarrow> (all_states ! (n + 1), all_messages ! (n + 1))\<close> \<open>valid_params (Suc n) i\<close> gr_implies_not0 list.size(3) state_length_invariant state_length_invariant_for_transition valid_params_def)
+
+  have "m \<in> all_messages ! n \<Longrightarrow> valid_params n (node_of (sender m)) \<and> valid_params n (node_of (receiver m))"
+    using \<open>\<And>m. \<lbrakk>valid_params n i; m \<in> all_messages ! n\<rbrakk> \<Longrightarrow> valid_params n (node_of (receiver m))\<close> \<open>\<And>m. \<lbrakk>valid_params n i; m \<in> all_messages ! n\<rbrakk> \<Longrightarrow> valid_params n (node_of (sender m))\<close> \<open>valid_params (Suc n) i\<close> valid_params_length_smaller by blast
+
+  have "length (all_states ! n) = number_of_nodes"
+    using \<open>(all_states ! n, all_messages ! n) \<rightarrow> (all_states ! (n + 1), all_messages ! (n + 1))\<close> \<open>valid_params (Suc n) i\<close> state_length_invariant state_length_invariant_for_transition by force
+  have "node_of (sender m) \<le> length (all_states ! n) \<and> node_of (receiver m) \<le> length (all_states ! n) \<Longrightarrow> valid_params (Suc n) (node_of (sender m)) \<and> valid_params (Suc n) (node_of (receiver m))"
+    apply (auto simp add: valid_params_def)
+    using \<open>valid_params (Suc n) i\<close> valid_params_def apply blast
+    using \<open>length (all_states ! n) = number_of_nodes\<close> \<open>m \<in> all_messages ! n \<Longrightarrow> valid_params n (node_of (sender m)) \<and> valid_params n (node_of (receiver m))\<close> \<open>m \<in> all_messages ! n \<or> node_of (sender m) < length (all_states ! n) \<and> node_of (receiver m) < length (all_states ! n)\<close> valid_params_def apply blast
+    using \<open>valid_params (Suc n) i\<close> raft.valid_params_def raft_axioms apply blast
+    using \<open>length (all_states ! n) = number_of_nodes\<close> \<open>m \<in> all_messages ! n \<Longrightarrow> valid_params n (node_of (sender m)) \<and> valid_params n (node_of (receiver m))\<close> \<open>m \<in> all_messages ! n \<or> node_of (sender m) < length (all_states ! n) \<and> node_of (receiver m) < length (all_states ! n)\<close> valid_params_def by blast
+
+  show "valid_params (Suc n) (node_of (sender m))" "valid_params (Suc n) (node_of (receiver m))"
+    apply (metis \<open>length (all_states ! n) = number_of_nodes\<close> \<open>m \<in> all_messages ! n \<Longrightarrow> valid_params n (node_of (sender m)) \<and> valid_params n (node_of (receiver m))\<close> \<open>m \<in> all_messages ! n \<or> node_of (sender m) < length (all_states ! n) \<and> node_of (receiver m) < length (all_states ! n)\<close> \<open>node_of (sender m) \<le> length (all_states ! n) \<and> node_of (receiver m) \<le> length (all_states ! n) \<Longrightarrow> valid_params (Suc n) (node_of (sender m)) \<and> valid_params (Suc n) (node_of (receiver m))\<close> nat_less_le valid_params_def)
+    by (metis \<open>length (all_states ! n) = number_of_nodes\<close> \<open>m \<in> all_messages ! n \<Longrightarrow> valid_params n (node_of (sender m)) \<and> valid_params n (node_of (receiver m))\<close> \<open>m \<in> all_messages ! n \<or> node_of (sender m) < length (all_states ! n) \<and> node_of (receiver m) < length (all_states ! n)\<close> \<open>node_of (sender m) \<le> length (all_states ! n) \<and> node_of (receiver m) \<le> length (all_states ! n) \<Longrightarrow> valid_params (Suc n) (node_of (sender m)) \<and> valid_params (Suc n) (node_of (receiver m))\<close> nat_less_le valid_params_def)
+qed
 
 lemma (in raft)
   assumes "number_of_nodes = 3"
